SIL-Parallel/SIL_Star_Sound.thy
@@ -1,7 +1,7 @@
 subsection \<open>Soundness and Completeness\<close>
 
 theory SIL_Star_Sound
-imports SIL_Star
+imports SIL_Star SIL_Single_Step_Sound
 begin
 
 subsubsection "Soundness"
@@ -16,7 +16,7 @@ assumes "\<And>n. \<turnstile> \<langle>Q (Suc n)\<rangle> c  \<langle>OK (Q n)\
   using assms
   apply (induct n arbitrary: s)
    apply (metis While small_step.IfFalse star.simps)
-  by (smt (verit, ccfv_threshold) Small_Step.WhileE Small_Step.post.distinct(1)
+  by (smt (verit, ccfv_threshold) Small_Step.WhileE Small_Step.sPost.distinct(1)
       com.distinct(13) final_def final_iff_SKIP seq_comp_sOK small_step.IfTrue star.step)
 
 lemma sil_while_sound_er:
@@ -29,12 +29,80 @@ lemma sil_while_sound_er:
   shows "\<exists>t. (WHILE b DO c, sOK s) \<rightarrow>* (SKIP, sER t) \<and> Q 0 t"
   using assms
   apply (induct m arbitrary: s)
-  apply (smt (verit) One_nat_def Small_Step.IfE Small_Step.WhileE Small_Step.post.distinct(1)
+  apply (smt (verit) One_nat_def Small_Step.IfE Small_Step.WhileE Small_Step.sPost.distinct(1)
       com.distinct(13,9) final_def final_iff_SKIP post_state.simps(1) seq_comp_sER star.simps)
   apply clarsimp
-  sorry
+  by (smt (verit, del_insts) Small_Step.WhileE Small_Step.sPost.distinct(1) com.distinct(13)
+      com.size_gen(2) final_def final_iff_SKIP seq_comp_sOK small_step.IfTrue star.simps
+      star.step)
 
+lemma sil_parL_sound_ok:
+  assumes h0: "c\<^sub>2 \<noteq> SKIP"
+  assumes h1: "\<turnstile> \<langle>P\<rangle> c\<^sub>1 \<leadsto> c\<^sub>1' \<langle>OK P'\<rangle>"
+  assumes h2: "\<turnstile> \<langle>P'\<rangle> c\<^sub>1' || c\<^sub>2 \<langle>Q\<rangle>"
+  assumes h3: "case Q of
+                 OK Q' \<Rightarrow> \<forall>s. P' s \<longrightarrow> (\<exists>t. (c\<^sub>1' || c\<^sub>2, sOK s) \<rightarrow>* (SKIP, sOK t) \<and> Q' t)
+               | ER Q' \<Rightarrow> \<forall>s. P' s \<longrightarrow> (\<exists>t. (c\<^sub>1' || c\<^sub>2, sOK s) \<rightarrow>* (SKIP, sER t) \<and> Q' t)"
+  shows "case Q of
+           OK Q' \<Rightarrow> \<forall>s. P s \<longrightarrow> (\<exists>t. (c\<^sub>1 || c\<^sub>2, sOK s) \<rightarrow>* (SKIP, sOK t) \<and> Q' t)
+         | ER Q' \<Rightarrow> \<forall>s. P s \<longrightarrow> (\<exists>t. (c\<^sub>1 || c\<^sub>2, sOK s) \<rightarrow>* (SKIP, sER t) \<and> Q' t)"
+proof (cases Q)
+  case (OK x)
+  have " \<forall>s. P s \<longrightarrow> (\<exists>t. (c\<^sub>1 || c\<^sub>2, sOK s) \<rightarrow> (c\<^sub>1' || c\<^sub>2, sOK t) \<and> P' t)"
+    using SIL_Single_Step_Valid_def h0 h1 sil_single_step_sound by fastforce
+  then show ?thesis
+    by (smt (verit, best) OK h3 post.simps(5) star.step)
+next
+  case (ER x)
+  have " \<forall>s. P s \<longrightarrow> (\<exists>t. (c\<^sub>1 || c\<^sub>2, sOK s) \<rightarrow> (c\<^sub>1' || c\<^sub>2, sOK t) \<and> P' t)"
+    using SIL_Single_Step_Valid_def h0 h1 sil_single_step_sound by fastforce
+  then show ?thesis
+    by (smt (verit, best) ER h3 post.simps(6) star.step)
+qed
 
+lemma sil_parR_sound_ok:
+  assumes h0: "c\<^sub>1 \<noteq> SKIP"
+  assumes h1: "\<turnstile> \<langle>P\<rangle> c\<^sub>2 \<leadsto> c\<^sub>2' \<langle>OK P'\<rangle>"
+  assumes h2: "\<turnstile> \<langle>P'\<rangle> c\<^sub>1 || c\<^sub>2' \<langle>Q\<rangle>"
+  assumes h3: "case Q of
+                 OK Q' \<Rightarrow> \<forall>s. P' s \<longrightarrow> (\<exists>t. (c\<^sub>1 || c\<^sub>2', sOK s) \<rightarrow>* (SKIP, sOK t) \<and> Q' t)
+               | ER Q' \<Rightarrow> \<forall>s. P' s \<longrightarrow> (\<exists>t. (c\<^sub>1 || c\<^sub>2', sOK s) \<rightarrow>* (SKIP, sER t) \<and> Q' t)"
+  shows "case Q of
+           OK Q' \<Rightarrow> \<forall>s. P s \<longrightarrow> (\<exists>t. (c\<^sub>1 || c\<^sub>2, sOK s) \<rightarrow>* (SKIP, sOK t) \<and> Q' t)
+         | ER Q' \<Rightarrow> \<forall>s. P s \<longrightarrow> (\<exists>t. (c\<^sub>1 || c\<^sub>2, sOK s) \<rightarrow>* (SKIP, sER t) \<and> Q' t)"
+proof (cases Q)
+  case (OK x)
+  have " \<forall>s. P s \<longrightarrow> (\<exists>t. (c\<^sub>1 || c\<^sub>2, sOK s) \<rightarrow> (c\<^sub>1 || c\<^sub>2', sOK t) \<and> P' t)"
+    using SIL_Single_Step_Valid_def h0 h1 sil_single_step_sound by fastforce
+  then show ?thesis
+    by (smt (verit, best) OK h3 post.simps(5) star.step)
+next
+  case (ER x)
+  have " \<forall>s. P s \<longrightarrow> (\<exists>t. (c\<^sub>1 || c\<^sub>2, sOK s) \<rightarrow> (c\<^sub>1 || c\<^sub>2', sOK t) \<and> P' t)"
+    using SIL_Single_Step_Valid_def h0 h1 sil_single_step_sound by fastforce
+  then show ?thesis
+    by (smt (verit, best) ER h3 post.simps(6) star.step)
+qed
+
+lemma sParL_sound_er:
+  assumes h0: "c\<^sub>2 \<noteq> SKIP"
+  assumes h1: "\<turnstile> \<langle>P\<rangle> c\<^sub>1 \<leadsto> c\<^sub>1' \<langle>ER Q\<rangle>"
+  shows "\<forall>s. P s \<longrightarrow> (\<exists>t. (c\<^sub>1 || c\<^sub>2, sOK s) \<rightarrow>* (SKIP, sER t) \<and> Q t)"
+proof-
+  have h0: "\<forall>s. P s \<longrightarrow> (\<exists>t. (c\<^sub>1 || c\<^sub>2, sOK s) \<rightarrow> (c\<^sub>1' || c\<^sub>2, sER t) \<and> Q t)" 
+    using SIL_Single_Step_Valid_def h0 h1 sil_single_step_sound by fastforce 
+  then show ?thesis  by (metis Er star.simps)
+qed
+
+lemma sParR_sound_er:
+  assumes h0: "c\<^sub>1 \<noteq> SKIP"
+  assumes h1: "\<turnstile> \<langle>P\<rangle> c\<^sub>2 \<leadsto> c\<^sub>2' \<langle>ER Q\<rangle>"
+  shows "\<forall>s. P s \<longrightarrow> (\<exists>t. (c\<^sub>1 || c\<^sub>2, sOK s) \<rightarrow>* (SKIP, sER t) \<and> Q t)"
+proof-
+  have h0: "\<forall>s. P s \<longrightarrow> (\<exists>t. (c\<^sub>1 || c\<^sub>2, sOK s) \<rightarrow> (c\<^sub>1 || c\<^sub>2', sER t) \<and> Q t)" 
+    using SIL_Single_Step_Valid_def h0 h1 sil_single_step_sound by fastforce 
+  then show ?thesis  by (metis Er star.simps)
+qed
 
 
 lemma sil_star_sound: 
@@ -101,9 +169,13 @@ lemma sil_star_sound:
         apply (smt (verit, best) case_prod_conv small_step.SelectND star.step)
        apply (simp add: sil_while_sound_ok)
       apply (smt (verit, ccfv_threshold) One_nat_def sil_while_sound_er)
-  sledgehammer
+     apply (simp add: sil_parL_sound_ok)
+    apply (simp add: sil_parR_sound_ok)
+   apply clarsimp 
+   apply (metis sParL_sound_er)
+  by (simp add: sParR_sound_er)
   
-
+end
 
                 
 
